Introduce a modal separation

src/dynamics.lean
@@ -1,10 +1,5 @@
 import syntax
 
-inductive val: exp -> Prop
-| int (n: ℤ): val (exp.int n)
-| true: val exp.true
-| false: val exp.false
-
 inductive steps: exp -> exp -> Prop
 | if_e1
     (e1: exp) (e1': exp) (e2: exp) (e3: exp):
@@ -12,7 +7,7 @@ inductive steps: exp -> exp -> Prop
     steps (exp.if_ e1 e2 e3) (exp.if_ e1' e2 e3)
 | if_e2
     (e2: exp) (e3: exp):
-    steps (exp.if_ exp.true e2 e3) e2
+    steps (exp.if_ (exp.pure val.true) e2 e3) e2
 | if_e3
     (e2: exp) (e3: exp):
-    steps (exp.if_ exp.false e2 e3) e3
+    steps (exp.if_ (exp.pure val.false) e2 e3) e3
