src/syntax.lean
@@ -5,8 +5,11 @@ inductive typ: Type
 | int: typ
 | bool: typ
 
+inductive val: Type
+| int: ℤ -> val
+| true: val
+| false: val
+
 inductive exp: Type
-| int: ℤ -> exp
-| true: exp
-| false: exp
+| pure: val -> exp
 | if_: exp -> exp -> exp -> exp
